wip: extraction should be ok

src/Main.Meta.fst
@@ -14,6 +14,7 @@ inline_for_extraction noextract
 let nb_arenas_nat : n:nat{n == US.v nb_arenas /\ n < pow2 32}
 = normalize_term (US.v nb_arenas)
 
+#push-options "--fuel 1 --ifuel 1 --z3rlimit 50"
 open FStar.Mul
 let total_nb_sc : n:nat{
   n == US.v nb_size_classes * US.v nb_arenas /\
@@ -23,8 +24,9 @@ let total_nb_sc : n:nat{
 assert_norm ((US.v nb_size_classes * US.v nb_arenas) < pow2 32);
 US.fits_u32_implies_fits (US.v nb_size_classes * US.v nb_arenas);
 normalize_term (US.v nb_size_classes * US.v nb_arenas)
+#pop-options
 
-#push-options "--fuel 1 --ifuel 1 --z3rlimit 100"
+#push-options "--fuel 1 --ifuel 1 --z3rlimit 200"
 /// Duplicating the list of size_classes sizes for each arena, which enables a simpler
 /// initialization directly using the mechanism in place for one arena
 [@@ reduce_attr]
@@ -44,6 +46,7 @@ let rec arena_sc_list'
   if i = nb_arenas_nat then acc
   else (
     List.append_length acc sc_list;
+    admit ();
     arena_sc_list' (i + 1) (acc `List.append` sc_list)
   )
 
@@ -69,7 +72,58 @@ let arena_sc_list = arena_sc_list' 0 []
 
 let sizes : sizes_t =
   normalize_term_spec arena_sc_list;
-  TLA.create #sc (normalize_term arena_sc_list)
+  TLA.create #sc_union (normalize_term arena_sc_list)
+
+type tuple4 = {
+  x: US.t;
+  y: US.t;
+  z: US.t;
+  w: US.t;
+}
+
+let gen_arena_sizes
+  (_:unit)
+  : Pure tuple4
+  (requires
+    True
+  )
+  (ensures fun r ->
+    hidden_pred sc_list_sc sc_list_ex
+      nb_size_classes
+      nb_size_classes_sc
+      nb_size_classes_sc_ex
+      r.y
+      r.z
+      r.w /\
+    hidden_pred2
+      nb_size_classes
+      r.x
+  )
+  =
+  admit ();
+  //assume (
+  //  US.fits (US.v arena_slab_region_size * US.v nb_arenas) /\
+  //  US.fits (US.v arena_md_bm_region_size * US.v nb_arenas) /\
+  //  US.fits (US.v arena_md_bm_region_b_size * US.v nb_arenas) /\
+  //  US.fits (US.v arena_md_region_size * US.v nb_arenas)
+  //);
+  let arena_slab_region_size
+    = US.mul sc_slab_region_size nb_size_classes in
+  let arena_md_bm_region_size
+    = US.mul (US.mul metadata_max 4sz) nb_size_classes_sc in
+  let arena_md_bm_region_b_size
+    = US.mul metadata_max_ex nb_size_classes_sc_ex in
+  let arena_md_region_size
+    = US.add
+      (US.mul metadata_max nb_size_classes_sc)
+      (US.mul metadata_max_ex nb_size_classes_sc_ex)
+  in
+  {
+    x = arena_slab_region_size;
+    y = arena_md_bm_region_size;
+    z = arena_md_bm_region_b_size;
+    w = arena_md_region_size
+  }
 
 #push-options "--z3rlimit 300 --fuel 0 --ifuel 0"
 let init
@@ -78,64 +132,38 @@ let init
   (fun _ -> emp)
   (fun _ r _ -> True)
   =
-  metadata_max_up_fits ();
-  US.fits_lte
-    (US.v nb_size_classes * US.v nb_arenas)
-    ((US.v metadata_max * U32.v page_size) * US.v nb_size_classes * US.v nb_arenas);
-  [@inline_let]
-  let n = nb_size_classes `US.mul` nb_arenas in
-  assert (
-    US.v n > 0 /\ US.v n >= US.v 1sz /\
-    US.v n == total_nb_sc /\
-    US.fits (US.v metadata_max * US.v (u32_to_sz page_size)) /\
-    US.fits (US.v metadata_max * US.v 4sz) /\
-    US.fits (US.v metadata_max * US.v (u32_to_sz page_size) * US.v n) /\
-    US.fits (US.v metadata_max * US.v 4sz * US.v n) /\
-    US.fits (US.v metadata_max * US.v n) /\
-    True
+  let arena_sizes = gen_arena_sizes () in
+  assume (
+    US.fits (US.v nb_size_classes * US.v nb_arenas) /\
+    US.fits (US.v arena_sizes.x * US.v nb_arenas) /\
+    US.fits (US.v arena_sizes.y * US.v nb_arenas) /\
+    US.fits (US.v arena_sizes.z * US.v nb_arenas) /\
+    US.fits (US.v arena_sizes.w * US.v nb_arenas)
   );
-  let slab_region = mmap_u8_init (US.mul (US.mul metadata_max (u32_to_sz page_size)) n) in
-  let md_bm_region = mmap_u64_init (US.mul (US.mul metadata_max 4sz) n) in
-  let md_region = mmap_cell_status_init (US.mul metadata_max n) in
+  let slab_region = mmap_u8_init (US.mul arena_sizes.x nb_arenas) in
+  let md_bm_region = mmap_u64_init (US.mul arena_sizes.y nb_arenas) in
+  let md_bm_region_b = mmap_bool_init (US.mul arena_sizes.z nb_arenas) in
+  let md_region = mmap_cell_status_init (US.mul arena_sizes.w nb_arenas) in
+  let size_classes = mmap_sc_init (US.mul nb_size_classes nb_arenas) in
 
-  Math.Lemmas.mul_zero_right_is_zero (US.v (US.mul metadata_max (u32_to_sz page_size)));
-  Math.Lemmas.mul_zero_right_is_zero (US.v (US.mul metadata_max 4sz));
-  Math.Lemmas.mul_zero_right_is_zero (US.v metadata_max);
-  A.ptr_shift_zero (A.ptr_of slab_region);
-  A.ptr_shift_zero (A.ptr_of md_bm_region);
-  A.ptr_shift_zero (A.ptr_of md_region);
-
-  change_equal_slprop
-    (A.varray slab_region)
-    (A.varray (A.split_r slab_region (US.mul (US.mul metadata_max (u32_to_sz page_size)) 0sz)));
-  change_equal_slprop
-    (A.varray md_bm_region)
-    (A.varray (A.split_r md_bm_region (US.mul (US.mul metadata_max 4sz) 0sz)));
-  change_equal_slprop
-    (A.varray md_region)
-    (A.varray (A.split_r md_region (US.mul metadata_max 0sz)));
-
-  assert (A.length (A.split_r slab_region (US.mul (US.mul metadata_max (u32_to_sz page_size)) 0sz)) == US.v metadata_max * US.v (u32_to_sz page_size) * US.v n);
-  assert (A.length (A.split_r md_bm_region (US.mul (US.mul metadata_max 4sz) 0sz)) == US.v metadata_max * 4 * US.v n);
-  assert (A.length (A.split_r md_region (US.mul metadata_max 0sz)) == US.v metadata_max * US.v n);
-
-  let size_classes = mmap_sc_init n in
-  //let sizes = mmap_sizes_init n in
-
-  init_size_classes arena_sc_list n slab_region md_bm_region md_region size_classes sizes;
+  init_all_arenas
+    sc_list_sc sc_list_ex
+    nb_size_classes_sc nb_size_classes_sc_ex
+    nb_size_classes
+    arena_sizes.x
+    arena_sizes.y
+    arena_sizes.z
+    arena_sizes.w
+    nb_arenas
+    slab_region
+    md_bm_region
+    md_bm_region_b
+    md_region
+    size_classes
+    sizes;
 
   let g_size_classes = gget (varray size_classes) in
-  //let g_sizes = gget (varray sizes) in
-
   let ro_perm = create_ro_array size_classes g_size_classes in
-  //let ro_sizes = create_ro_array sizes g_sizes in
-
-  drop (A.varray (A.split_r slab_region (US.mul (US.mul metadata_max (u32_to_sz page_size))
-    n)));
-  drop (A.varray (A.split_r md_bm_region (US.mul (US.mul metadata_max 4sz)
-    n)));
-  drop (A.varray (A.split_r md_region (US.mul metadata_max
-   n)));
 
   [@inline_let]
   let s : size_classes_all = {
@@ -165,18 +193,20 @@ let slab_malloc_one (i:US.t{US.v i < total_nb_sc}) (bytes: U32.t)
   (array U8.t)
   emp (fun r -> null_or_varray r)
   (requires fun _ ->
-    U32.v bytes <= U32.v (Seq.index (G.reveal sc_all.g_size_classes) (US.v i)).data.size
+    U32.v bytes <= U32.v (get_u32 (Seq.index (G.reveal sc_all.g_size_classes) (US.v i)).data.size)
   )
   (ensures fun _ r _ ->
-    let size = (Seq.index sc_all.g_size_classes (US.v i)).data.size in
+    let size = get_u32 (Seq.index sc_all.g_size_classes (US.v i)).data.size in
+    U32.v size > 0 /\
     not (is_null r) ==> (
-      A.length r == U32.v (Seq.index (G.reveal sc_all.g_size_classes) (US.v i)).data.size /\
+      A.length r == U32.v size /\
       A.length r >= U32.v bytes /\
-      array_u8_alignment r 16ul /\
-      ((U32.v page_size) % (U32.v size) == 0 ==> array_u8_alignment r size)
+      array_u8_alignment r 16sz /\
+      ((U32.v page_size) % (U32.v size) == 0 ==> array_u8_alignment r (u32_to_sz size))
     )
   )
   =
+  admit ();
   let sc = index sc_all.ro_perm i in
   L.acquire sc.lock;
   let sc = index sc_all.ro_perm i in
@@ -196,7 +226,7 @@ let cons_implies_positive_length (#a: Type) (l: list a)
 
 #push-options "--fuel 0 --ifuel 0 --z3rlimit 100 --query_stats"
 let aux_lemma
-  (l:list sc{List.length l <= length sc_all.size_classes /\ Cons? l})
+  (l:list sc_union{List.length l <= length sc_all.size_classes /\ Cons? l})
   (i:US.t{US.v i + List.length l == US.v nb_size_classes})
   (arena_id:US.t{US.v arena_id < US.v nb_arenas})
   : Lemma
@@ -233,7 +263,7 @@ let aux_lemma
 
 #restart-solver
 
-#push-options "--fuel 1 --ifuel 1 --z3rlimit 100"
+#push-options "--fuel 1 --ifuel 1 --z3rlimit 200"
 /// A wrapper around slab_malloc' that performs dispatch in the size classes
 /// for arena [arena_id] in a generic way.
 /// The list argument is not actually used, it just serves
@@ -241,7 +271,7 @@ let aux_lemma
 [@@ reduce_attr]
 noextract
 let rec slab_malloc_i
-  (l:list sc{List.length l <= length sc_all.size_classes})
+  (l:list sc_union{List.length l <= length sc_all.size_classes})
   (i:US.t{US.v i + List.length l == US.v nb_size_classes})
   (arena_id:US.t{US.v arena_id < US.v nb_arenas})
   bytes
@@ -254,7 +284,7 @@ let rec slab_malloc_i
       = h1 (null_or_varray r) in
     not (is_null r) ==> (
       A.length r >= U32.v bytes /\
-      array_u8_alignment r 16ul /\
+      array_u8_alignment r 16sz /\
       Seq.length s >= 2
     )
   )
@@ -263,7 +293,8 @@ let rec slab_malloc_i
     | hd::tl ->
       aux_lemma l i arena_id;
       [@inline_let] let idx = (arena_id `US.mul` nb_size_classes) `US.add` i in
-      let size = TLA.get sizes idx in
+      let size = get_u32 (TLA.get sizes idx) in
+      admit ();
       if bytes `U32.lte` size then
         slab_malloc_one idx bytes
       else
@@ -306,7 +337,7 @@ let set_canary
 [@@ reduce_attr]
 noextract
 let rec slab_malloc_canary_i
-  (l:list sc{List.length l <= length sc_all.size_classes})
+  (l:list sc_union{List.length l <= length sc_all.size_classes})
   (i:US.t{US.v i + List.length l == US.v nb_size_classes})
   (arena_id:US.t{US.v arena_id < US.v nb_arenas})
   bytes
@@ -319,7 +350,7 @@ let rec slab_malloc_canary_i
       = h1 (null_or_varray r) in
     not (is_null r) ==> (
       A.length r >= U32.v bytes /\
-      array_u8_alignment r 16ul /\
+      array_u8_alignment r 16sz /\
       Seq.length s >= 2 /\
       Seq.index s (A.length r - 2) == slab_canaries_magic1 /\
       Seq.index s (A.length r - 1) == slab_canaries_magic2
@@ -330,7 +361,8 @@ let rec slab_malloc_canary_i
     | hd::tl ->
       aux_lemma l i arena_id;
       [@inline_let] let idx = (arena_id `US.mul` nb_size_classes) `US.add` i in
-      let size = TLA.get sizes idx in
+      let size = get_u32 (TLA.get sizes idx) in
+      admit ();
       if bytes `U32.lte` (size `U32.sub` 2ul) then
         let ptr = slab_malloc_one idx bytes in
         set_canary ptr size;
@@ -341,10 +373,13 @@ let rec slab_malloc_canary_i
 
 #push-options "--fuel 1 --ifuel 1 --z3rlimit 100"
 let slab_malloc arena_id bytes =
-  if enable_slab_canaries_malloc then
+  if enable_slab_canaries_malloc then (
+    admit ();
     (slab_malloc_canary_i sc_list 0sz) arena_id bytes
-  else
+  ) else (
+    admit ();
     (slab_malloc_i sc_list 0sz) arena_id bytes
+  )
 #pop-options
 
 #restart-solver
@@ -359,7 +394,7 @@ open MiscArith
 [@@ reduce_attr]
 noextract
 let rec slab_aligned_alloc_i
-  (l:list sc{List.length l <= length sc_all.size_classes})
+  (l:list sc_union{List.length l <= length sc_all.size_classes})
   (i:US.t{US.v i + List.length l == US.v nb_size_classes})
   (arena_id:US.t{US.v arena_id < US.v nb_arenas})
   (alignment: (v:U32.t{U32.v v > 0 /\ (U32.v page_size) % (U32.v v) = 0}))
@@ -373,8 +408,8 @@ let rec slab_aligned_alloc_i
       = h1 (null_or_varray r) in
     not (is_null r) ==> (
       A.length r >= U32.v bytes /\
-      array_u8_alignment r 16ul /\
-      array_u8_alignment r alignment /\
+      array_u8_alignment r 16sz /\
+      array_u8_alignment r (u32_to_sz alignment) /\
       Seq.length s >= 2
     )
   )
@@ -383,17 +418,18 @@ let rec slab_aligned_alloc_i
     | hd::tl ->
       aux_lemma l i arena_id;
       [@inline_let] let idx = (arena_id `US.mul` nb_size_classes) `US.add` i in
-      let size = TLA.get sizes idx in
+      let size = get_u32 (TLA.get sizes idx) in
+      admit ();
       let b = U32.eq (U32.rem page_size size) 0ul in
       if b && bytes `U32.lte` size && alignment `U32.lte` size then (
         let r = slab_malloc_one idx bytes in
-        let size_ = G.hide (Seq.index sc_all.g_size_classes (US.v idx)).data.size in
+        let size_ = G.hide (get_u32 (Seq.index sc_all.g_size_classes (US.v idx)).data.size) in
         assert (G.reveal size_ = size);
         assert ((U32.v page_size) % (U32.v (G.reveal size_ )) = 0);
         assert_norm (U32.v page_size = pow2 12);
         alignment_lemma (U32.v page_size) 12 (U32.v alignment) (U32.v size);
         assert (U32.v size % U32.v alignment = 0);
-        array_u8_alignment_lemma2 r size alignment;
+        array_u8_alignment_lemma2 r (u32_to_sz size) (u32_to_sz alignment);
         return r
       ) else (
         slab_aligned_alloc_i tl (i `US.add` 1sz) arena_id alignment bytes
@@ -407,7 +443,7 @@ let rec slab_aligned_alloc_i
 [@@ reduce_attr]
 noextract
 let rec slab_aligned_alloc_canary_i
-  (l:list sc{List.length l <= length sc_all.size_classes})
+  (l:list sc_union{List.length l <= length sc_all.size_classes})
   (i:US.t{US.v i + List.length l == US.v nb_size_classes})
   (arena_id:US.t{US.v arena_id < US.v nb_arenas})
   (alignment: (v:U32.t{U32.v v > 0 /\ (U32.v page_size) % (U32.v v) = 0}))
@@ -421,8 +457,8 @@ let rec slab_aligned_alloc_canary_i
       = h1 (null_or_varray r) in
     not (is_null r) ==> (
       A.length r >= U32.v bytes /\
-      array_u8_alignment r 16ul /\
-      array_u8_alignment r alignment /\
+      array_u8_alignment r 16sz /\
+      array_u8_alignment r (u32_to_sz alignment) /\
       Seq.length s >= 2 /\
       Seq.index s (A.length r - 2) == slab_canaries_magic1 /\
       Seq.index s (A.length r - 1) == slab_canaries_magic2
@@ -433,17 +469,18 @@ let rec slab_aligned_alloc_canary_i
     | hd::tl ->
       aux_lemma l i arena_id;
       [@inline_let] let idx = (arena_id `US.mul` nb_size_classes) `US.add` i in
-      let size = TLA.get sizes idx in
+      let size = get_u32 (TLA.get sizes idx) in
+      admit ();
       let b = U32.eq (U32.rem page_size size) 0ul in
       if b && bytes `U32.lte` (size `U32.sub` 2ul) && alignment `U32.lte` size then (
         let ptr = slab_malloc_one idx bytes in
-        let size_ = G.hide (Seq.index sc_all.g_size_classes (US.v idx)).data.size in
+        let size_ = G.hide (get_u32 (Seq.index sc_all.g_size_classes (US.v idx)).data.size) in
         assert (G.reveal size_ = size);
         assert ((U32.v page_size) % (U32.v (G.reveal size_ )) = 0);
         assert_norm (U32.v page_size = pow2 12);
         alignment_lemma (U32.v page_size) 12 (U32.v alignment) (U32.v size);
         assert (U32.v size % U32.v alignment = 0);
-        array_u8_alignment_lemma2 ptr size alignment;
+        array_u8_alignment_lemma2 ptr (u32_to_sz size) (u32_to_sz alignment);
         set_canary ptr size;
         return ptr
       ) else (
@@ -453,6 +490,7 @@ let rec slab_aligned_alloc_canary_i
 
 #push-options "--fuel 1 --ifuel 1 --z3rlimit 100"
 let slab_aligned_alloc arena_id alignment bytes =
+  admit ();
   if enable_slab_canaries_malloc then
     (slab_aligned_alloc_canary_i sc_list 0sz) arena_id alignment bytes
   else
@@ -473,8 +511,8 @@ let slab_free' (i:US.t{US.v i < US.v nb_size_classes * US.v nb_arenas}) (ptr: ar
     same_base_array ptr sc.data.slab_region /\
     0 <= diff' /\
     diff' < US.v slab_size /\
-    (diff' % U32.v page_size) % U32.v sc.data.size == 0 /\
-    A.length ptr == U32.v sc.data.size /\
+    (diff' % U32.v page_size) % U32.v (get_u32 sc.data.size) == 0 /\
+    A.length ptr == U32.v (get_u32 sc.data.size) /\
     US.v diff = diff')
   (ensures fun h0 _ h1 -> True)
   =
@@ -499,14 +537,14 @@ let within_size_class_i (ptr:A.array U8.t) (sc: size_class_struct) : prop = (
   A.offset (A.ptr_of ptr) - A.offset (A.ptr_of (G.reveal sc.slab_region)) >= 0 /\
   A.offset (A.ptr_of ptr) - A.offset (A.ptr_of (G.reveal sc.slab_region)) < US.v slab_size /\
   // and it is aligned on the slots
-  ((A.offset (A.ptr_of ptr) - A.offset (A.ptr_of (G.reveal sc.slab_region))) % U32.v page_size) % U32.v sc.size = 0) ==>
+  ((A.offset (A.ptr_of ptr) - A.offset (A.ptr_of (G.reveal sc.slab_region))) % U32.v page_size) % U32.v (get_u32 sc.size) = 0) ==>
     // then its length is the length of a slot
-    A.length ptr == U32.v sc.size
+    A.length ptr == U32.v (get_u32 sc.size)
 
 #push-options "--fuel 1 --ifuel 1 --z3rlimit 150"
 /// Elimination lemma for `within_size_class_i`, triggering F* to prove the precondition
 /// of the implication
-let elim_within_size_class_i (ptr:A.array U8.t) (i:nat{i < Seq.length sc_all.g_size_classes}) (size:sc)
+let elim_within_size_class_i (ptr:A.array U8.t) (i:nat{i < Seq.length sc_all.g_size_classes}) (size:sc_union)
   : Lemma
   (requires (
     let sc : size_class = G.reveal (Seq.index sc_all.g_size_classes i) in
@@ -515,13 +553,14 @@ let elim_within_size_class_i (ptr:A.array U8.t) (i:nat{i < Seq.length sc_all.g_s
     same_base_array sc.data.slab_region ptr /\
     A.offset (A.ptr_of ptr) - A.offset (ptr_of (G.reveal sc.data.slab_region)) >= 0 /\
     A.offset (A.ptr_of ptr) - A.offset (ptr_of (G.reveal sc.data.slab_region)) < US.v slab_size /\
-    ((A.offset (A.ptr_of ptr) - A.offset (ptr_of (G.reveal sc_all.slab_region))) % U32.v page_size) % U32.v size = 0))
+    ((A.offset (A.ptr_of ptr) - A.offset (ptr_of (G.reveal sc_all.slab_region))) % U32.v page_size) % U32.v (get_u32 size) = 0))
   (ensures (
     let sc : size_class = G.reveal (Seq.index sc_all.g_size_classes i) in
-    ((A.offset (A.ptr_of ptr) - A.offset (ptr_of (G.reveal sc.data.slab_region))) % U32.v page_size) % U32.v size = 0 /\
-    A.length ptr == U32.v size
+    ((A.offset (A.ptr_of ptr) - A.offset (ptr_of (G.reveal sc.data.slab_region))) % U32.v page_size) % U32.v (get_u32 size) = 0 /\
+    A.length ptr == U32.v (get_u32 size)
   ))
   =
+  admit ();
   let sc : size_class = G.reveal (Seq.index sc_all.g_size_classes i) in
   let off_ptr = A.offset (A.ptr_of ptr) in
   let off1 = A.offset (A.ptr_of (G.reveal sc_all.slab_region)) in
@@ -571,10 +610,11 @@ let slab_getsize ptr =
     ptr
     (A.split_l sc_all.slab_region 0sz) in
   let diff_sz = UP.ptrdifft_to_sizet diff in
+  admit ();
   let index = US.div diff_sz slab_size in
   lemma_div_lt (US.v slab_size) (US.v nb_size_classes) (US.v nb_arenas) (US.v diff_sz);
   assert (US.v index < US.v nb_size_classes * US.v nb_arenas);
-  let size = TLA.get sizes index in
+  let size = get_u32 (TLA.get sizes index) in
   let rem_slab = US.rem diff_sz slab_size in
   let rem_slot = US.rem diff_sz (u32_to_sz page_size) in
   // TODO: some refactor needed wrt SlotsFree
@@ -588,7 +628,7 @@ let slab_getsize ptr =
     mod_lt diff_sz (u32_to_sz page_size);
     assert (US.v rem_slot == (A.offset (A.ptr_of ptr) - A.offset (A.ptr_of sc_all.slab_region)) % (U32.v page_size));
     mod_lt rem_slot (US.uint32_to_sizet size);
-    (**) elim_within_size_class_i ptr (US.v index) size;
+    //(**) elim_within_size_class_i ptr (US.v index) size;
     (**) assert (A.length ptr == U32.v size);
     if enable_slab_canaries_malloc then
       return (US.uint32_to_sizet (size `U32.sub` 2ul))
@@ -615,10 +655,11 @@ let slab_free ptr =
     ptr
     (A.split_l sc_all.slab_region 0sz) in
   let diff_sz = UP.ptrdifft_to_sizet diff in
+  admit ();
   let index = US.div diff_sz slab_size in
   lemma_div_lt (US.v slab_size) (US.v nb_size_classes) (US.v nb_arenas) (US.v diff_sz);
   assert (US.v index < US.v nb_size_classes * US.v nb_arenas);
-  let size = TLA.get sizes index in
+  let size = get_u32 (TLA.get sizes index) in
   let rem_slab = US.rem diff_sz slab_size in
   let rem_slot = US.rem diff_sz (u32_to_sz page_size) in
   // TODO: some refactor needed wrt SlotsFree
@@ -632,7 +673,7 @@ let slab_free ptr =
     mod_lt diff_sz (u32_to_sz page_size);
     assert (US.v rem_slot == (A.offset (A.ptr_of ptr) - A.offset (A.ptr_of sc_all.slab_region)) % (U32.v page_size));
     mod_lt rem_slot (US.uint32_to_sizet size);
-    (**) elim_within_size_class_i ptr (US.v index) size;
+    //(**) elim_within_size_class_i ptr (US.v index) size;
     (**) assert (A.length ptr == U32.v size);
     if enable_slab_canaries_free then (
       enable_slab_canaries_lemma ();
