src/LargeAlloc.fst
@@ -227,7 +227,7 @@ let large_malloc_aux
       (enable_slab_canaries_malloc ==> A.length r == US.v size + 2) /\
       (not enable_slab_canaries_malloc ==> A.length r == US.v size) /\
       A.is_full_array r /\
-      array_u8_alignment r page_size /\
+      array_u8_alignment r (u32_to_sz page_size) /\
       zf_u8 s /\
       not (Spec.mem (spec_convert cmp) t (r, size)) /\
       Spec.mem (spec_convert cmp) t' (r, size)
@@ -401,7 +401,7 @@ let large_malloc (size: US.t)
     not (A.is_null ptr) ==> (
       (enable_slab_canaries_malloc ==> A.length ptr == US.v size + 2) /\
       (not enable_slab_canaries_malloc ==> A.length ptr == US.v size) /\
-      array_u8_alignment ptr page_size /\
+      array_u8_alignment ptr (u32_to_sz page_size) /\
       A.is_full_array ptr /\
       zf_u8 s
     )
