src/Mman.fst
@@ -54,6 +54,17 @@ assume val mmap_cell_status_init (len: US.t)
       A.is_full_array r
     )
 
+assume val mmap_bool_init (len: US.t)
+  : Steel (array bool)
+     emp
+    (fun r -> A.varray r)
+    (fun _ -> US.v len > 0)
+    (fun _ r h1 ->
+      A.length r == US.v len /\
+      A.is_full_array r /\
+      A.asel r h1 == Seq.create (US.v len) false
+    )
+
 assume val mmap_ptr_us_init (_:unit)
   : SteelT (R.ref US.t)
     emp
@@ -91,15 +102,15 @@ assume val mmap_sc_init (len: US.t)
       A.is_full_array r
     )
 
-assume val mmap_sizes_init (len: US.t)
-  : Steel (array sc)
-     emp
-    (fun r -> A.varray r)
-    (fun _ -> US.v len > 0)
-    (fun _ r h1 ->
-      A.length r == US.v len /\
-      A.is_full_array r
-    )
+//assume val mmap_sizes_init (len: US.t)
+//  : Steel (array sc)
+//     emp
+//    (fun r -> A.varray r)
+//    (fun _ -> US.v len > 0)
+//    (fun _ r h1 ->
+//      A.length r == US.v len /\
+//      A.is_full_array r
+//    )
 
 // used in src/LargeAlloc.fst
 // mmap_ptr_metadata
